Use `Nat` instead of `USize`

src/native/buffer.c
@@ -2,25 +2,29 @@
 #include <string.h>
 #include "include/lean_pod.h"
 
-LEAN_EXPORT lean_obj_res lean_pod_Buffer_allocate(size_t sz) {
+LEAN_EXPORT lean_obj_res lean_pod_Buffer_allocate(b_lean_obj_arg sz_nat) {
+    size_t sz = lean_usize_of_nat(sz_nat);
     return lean_pod_Buffer_wrap(malloc(sz), free);
 }
 
-LEAN_EXPORT lean_obj_res lean_pod_Buffer_allocateClear(size_t sz) {
+LEAN_EXPORT lean_obj_res lean_pod_Buffer_allocateClear(b_lean_obj_arg sz_nat) {
+    size_t sz = lean_usize_of_nat(sz_nat);
     return lean_pod_Buffer_wrap(calloc(1, sz), free);
 }
 
-LEAN_EXPORT lean_obj_res lean_pod_Buffer_view(size_t sz, b_lean_obj_arg align, lean_obj_arg buf) {
+LEAN_EXPORT lean_obj_res lean_pod_Buffer_view(b_lean_obj_arg sz_nat, b_lean_obj_arg align, lean_obj_arg buf) {
+    size_t sz = lean_usize_of_nat(sz_nat);
     return lean_pod_BytesView_wrap(lean_pod_Buffer_unwrap(buf)->data, buf);
 }
 
-LEAN_EXPORT lean_obj_res lean_pod_Buffer_withRef(size_t sz, b_lean_obj_arg align, lean_obj_arg buf, lean_obj_arg f) {
+LEAN_EXPORT lean_obj_res lean_pod_Buffer_withRef(b_lean_obj_arg sz_nat, b_lean_obj_arg align, lean_obj_arg buf, lean_obj_arg f) {
+    size_t sz = lean_usize_of_nat(sz_nat);
     lean_object* buf_res;
     if(LEAN_LIKELY(lean_is_exclusive(buf))) {
         buf_res = buf;
     }
     else {
-        buf_res = lean_pod_Buffer_allocate(sz);
+        buf_res = lean_pod_Buffer_wrap(malloc(sz), free);
         memcpy(lean_pod_Buffer_unwrap(buf_res)->data, lean_pod_Buffer_unwrap(buf)->data, sz);
         lean_dec_ref(buf);
     }
