src/native/bytes_ref.c
@@ -50,19 +50,32 @@ LEAN_EXPORT lean_obj_res lean_pod_ByteArray_withRefEx(lean_obj_arg ba, lean_obj_
     return exok;
 }
 
-LEAN_EXPORT lean_obj_res lean_pod_BytesRef_weaken(uint8_t mut, size_t sz, b_lean_obj_arg a0, b_lean_obj_arg a1, lean_obj_arg br) {
+LEAN_EXPORT lean_obj_res lean_pod_BytesRef_weaken(
+    uint8_t mut, b_lean_obj_arg sz, b_lean_obj_arg a0, b_lean_obj_arg a1,
+    lean_obj_arg br
+) {
     return br;
 }
 
-LEAN_EXPORT lean_obj_res lean_pod_BytesRef_imm(uint8_t mut, size_t sz, b_lean_obj_arg a, lean_obj_arg br) {
+LEAN_EXPORT lean_obj_res lean_pod_BytesRef_imm(
+    uint8_t mut, b_lean_obj_arg sz, b_lean_obj_arg a,
+    lean_obj_arg br
+) {
     return br;
 }
 
-LEAN_EXPORT lean_obj_res lean_pod_BytesRef_take(uint8_t mut, size_t size, b_lean_obj_arg a, lean_obj_arg br, size_t count) {
+LEAN_EXPORT lean_obj_res lean_pod_BytesRef_take(
+    uint8_t mut, b_lean_obj_arg sz, b_lean_obj_arg a,
+    lean_obj_arg br, b_lean_obj_arg count
+) {
     return br;
 }
 
-LEAN_EXPORT lean_obj_res lean_pod_BytesRef_drop(uint8_t mut, size_t size, b_lean_obj_arg a, lean_obj_arg br, size_t count) {
+LEAN_EXPORT lean_obj_res lean_pod_BytesRef_drop(
+    uint8_t mut, b_lean_obj_arg sz, b_lean_obj_arg a,
+    lean_obj_arg br, b_lean_obj_arg count_nat
+) {
+    size_t count = lean_usize_of_nat(count_nat);
     if(lean_is_exclusive(br)) {
         lean_to_external(br)->m_data += count;
         return br;
@@ -71,20 +84,28 @@ LEAN_EXPORT lean_obj_res lean_pod_BytesRef_drop(uint8_t mut, size_t size, b_lean
     return lean_pod_BytesRef_wrap(lean_to_external(br)->m_data + count);
 }
 
-LEAN_EXPORT lean_obj_res lean_pod_BytesRef_slice(uint8_t mut, size_t sz, b_lean_obj_arg a, lean_obj_arg br, size_t start, size_t length) {
+LEAN_EXPORT lean_obj_res lean_pod_BytesRef_slice(
+    uint8_t mut, b_lean_obj_arg sz, b_lean_obj_arg a,
+    lean_obj_arg br, b_lean_obj_arg start, b_lean_obj_arg length
+) {
     return lean_pod_BytesRef_drop(mut, sz, a, br, start);
 }
 
-LEAN_EXPORT lean_obj_res lean_pod_BytesRef_toByteArray(uint8_t mut, size_t sz, b_lean_obj_arg a, b_lean_obj_arg br, lean_obj_arg token) {
+LEAN_EXPORT lean_obj_res lean_pod_BytesRef_toByteArray(
+    uint8_t mut, b_lean_obj_arg sz_nat, b_lean_obj_arg a,
+    b_lean_obj_arg br, lean_obj_arg token
+) {
+    size_t sz = lean_usize_of_nat(sz_nat);
     lean_object* arr = lean_alloc_sarray(1, sz, sz);
     memcpy(lean_sarray_cptr(arr), lean_pod_BytesRef_unwrap(br), sz);
     return lean_io_result_mk_ok(arr);
 }
 
 LEAN_EXPORT lean_obj_res lean_pod_BytesRef_copyView(
-    size_t sz, b_lean_obj_arg a1, b_lean_obj_arg a2,
+    b_lean_obj_arg sz_nat, b_lean_obj_arg a1, b_lean_obj_arg a2,
     b_lean_obj_arg dst, b_lean_obj_arg src, lean_obj_arg token
 ) {
+    size_t sz = lean_usize_of_nat(sz_nat);
     memcpy(lean_pod_BytesRef_unwrap(dst), lean_pod_BytesView_unwrap(src)->ptr, sz);
     return lean_io_result_mk_ok(lean_box(0));
 }
