src/native/bytes_view.c
@@ -5,15 +5,25 @@ LEAN_EXPORT lean_obj_res lean_pod_ByteArray_view(lean_obj_arg ba) {
     return lean_pod_BytesView_wrap(lean_sarray_cptr(ba), ba);
 }
 
-LEAN_EXPORT lean_obj_res lean_pod_BytesView_weaken(size_t sz, b_lean_obj_arg a0, b_lean_obj_arg a1, lean_obj_arg bv) {
+LEAN_EXPORT lean_obj_res lean_pod_BytesView_weaken(
+    b_lean_obj_arg sz, b_lean_obj_arg a0, b_lean_obj_arg a1,
+    lean_obj_arg bv
+) {
     return bv;
 }
 
-LEAN_EXPORT lean_obj_res lean_pod_BytesView_take(size_t size, b_lean_obj_arg a, lean_obj_arg bv, size_t count) {
+LEAN_EXPORT lean_obj_res lean_pod_BytesView_take(
+    b_lean_obj_arg sz, b_lean_obj_arg a,
+    lean_obj_arg bv, b_lean_obj_arg count
+) {
     return bv;
 }
 
-LEAN_EXPORT lean_obj_res lean_pod_BytesView_drop(size_t size, b_lean_obj_arg a, lean_obj_arg bv_w, size_t count) {
+LEAN_EXPORT lean_obj_res lean_pod_BytesView_drop(
+    b_lean_obj_arg sz, b_lean_obj_arg a,
+    lean_obj_arg bv_w, b_lean_obj_arg count_nat
+) {
+    size_t count = lean_usize_of_nat(count_nat);
     lean_pod_BytesView* bv = lean_pod_BytesView_unwrap(bv_w);
     if(lean_is_exclusive(bv_w)) {
         bv->ptr += count;
@@ -23,11 +33,18 @@ LEAN_EXPORT lean_obj_res lean_pod_BytesView_drop(size_t size, b_lean_obj_arg a, 
     return lean_pod_BytesView_wrap(bv->ptr + count, bv->owner);
 }
 
-LEAN_EXPORT lean_obj_res lean_pod_BytesView_slice(size_t sz, b_lean_obj_arg a, lean_obj_arg bv_w, size_t start, size_t length) {
+LEAN_EXPORT lean_obj_res lean_pod_BytesView_slice(
+    b_lean_obj_arg sz, b_lean_obj_arg a,
+    lean_obj_arg bv_w, b_lean_obj_arg start, b_lean_obj_arg length
+) {
     return lean_pod_BytesView_drop(sz, a, bv_w, start);
 }
 
-LEAN_EXPORT lean_obj_res lean_pod_BytesView_toByteArray(size_t sz, b_lean_obj_arg a, b_lean_obj_arg bv) {
+LEAN_EXPORT lean_obj_res lean_pod_BytesView_toByteArray(
+    b_lean_obj_arg sz_nat, b_lean_obj_arg a,
+    b_lean_obj_arg bv
+) {
+    size_t sz = lean_usize_of_nat(sz_nat);
     lean_object* arr = lean_alloc_sarray(1, sz, sz);
     memcpy(lean_sarray_cptr(arr), lean_pod_BytesView_unwrap(bv)->ptr, sz);
     return arr;
