src/native/instances.c
@@ -20,12 +20,14 @@ LEAN_EXPORT lean_obj_res lean_pod_readBytesRefUnal_##ltyp(b_lean_obj_arg a, b_le
     memcpy(&value, lean_pod_BytesRef_unwrap(br), sizeof(ctyp));\
     return lean_io_result_mk_ok(box(value));\
 }\
-LEAN_EXPORT lean_obj_res lean_pod_readBytesRefOffUnal_##ltyp(size_t sz, b_lean_obj_arg a, b_lean_obj_arg br, size_t i, lean_obj_arg st) {\
+LEAN_EXPORT lean_obj_res lean_pod_readBytesRefOffUnal_##ltyp(b_lean_obj_arg sz, b_lean_obj_arg a, b_lean_obj_arg br, b_lean_obj_arg i_nat, lean_obj_arg st) {\
+    size_t i = lean_usize_of_nat(i_nat);\
     ctyp value;\
     memcpy(&value, lean_pod_BytesRef_unwrap(br) + i, sizeof(ctyp));\
     return lean_io_result_mk_ok(box(value));\
 }\
-LEAN_EXPORT lean_obj_res lean_pod_readBytesRefOffElUnal_##ltyp(size_t sz, b_lean_obj_arg a, b_lean_obj_arg br, size_t i, lean_obj_arg st) {\
+LEAN_EXPORT lean_obj_res lean_pod_readBytesRefOffElUnal_##ltyp(b_lean_obj_arg sz, b_lean_obj_arg a, b_lean_obj_arg br, b_lean_obj_arg i_nat, lean_obj_arg st) {\
+    size_t i = lean_usize_of_nat(i_nat);\
     ctyp value;\
     memcpy(&value, lean_pod_BytesRef_unwrap(br) + i * sizeof(ctyp), sizeof(ctyp));\
     return lean_io_result_mk_ok(box(value));\
@@ -36,13 +38,15 @@ LEAN_EXPORT lean_obj_res lean_pod_readBytesRef_##ltyp(b_lean_obj_arg br, lean_ob
     memcpy(&value, LEAN_POD_ASSUME_ALIGNED(p, ctyp), sizeof(ctyp));\
     return lean_io_result_mk_ok(box(value));\
 }\
-LEAN_EXPORT lean_obj_res lean_pod_readBytesRefOff_##ltyp(size_t sz, b_lean_obj_arg a, b_lean_obj_arg br, size_t i, lean_obj_arg st) {\
+LEAN_EXPORT lean_obj_res lean_pod_readBytesRefOff_##ltyp(b_lean_obj_arg sz, b_lean_obj_arg a, b_lean_obj_arg br, b_lean_obj_arg i_nat, lean_obj_arg st) {\
+    size_t i = lean_usize_of_nat(i_nat);\
     ctyp value;\
     unsigned char* p = lean_pod_BytesRef_unwrap(br) + i;\
     memcpy(&value, LEAN_POD_ASSUME_ALIGNED(p, ctyp), sizeof(ctyp));\
     return lean_io_result_mk_ok(box(value));\
 }\
-LEAN_EXPORT lean_obj_res lean_pod_readBytesRefOffEl_##ltyp(size_t sz, b_lean_obj_arg br, size_t i, lean_obj_arg st) {\
+LEAN_EXPORT lean_obj_res lean_pod_readBytesRefOffEl_##ltyp(b_lean_obj_arg sz, b_lean_obj_arg br, b_lean_obj_arg i_nat, lean_obj_arg st) {\
+    size_t i = lean_usize_of_nat(i_nat);\
     ctyp value;\
     unsigned char* p = lean_pod_BytesRef_unwrap(br) + i * sizeof(ctyp);\
     memcpy(&value, LEAN_POD_ASSUME_ALIGNED(p, ctyp), sizeof(ctyp));\
@@ -54,12 +58,14 @@ LEAN_EXPORT ctyp lean_pod_readBytesViewUnal_##ltyp(b_lean_obj_arg a, b_lean_obj_
     memcpy(&value, lean_pod_BytesView_unwrap(bv)->ptr, sizeof(ctyp));\
     return value;\
 }\
-LEAN_EXPORT ctyp lean_pod_readBytesViewOffUnal_##ltyp(size_t sz, b_lean_obj_arg a, b_lean_obj_arg bv, size_t i) {\
+LEAN_EXPORT ctyp lean_pod_readBytesViewOffUnal_##ltyp(b_lean_obj_arg sz, b_lean_obj_arg a, b_lean_obj_arg bv, b_lean_obj_arg i_nat) {\
+    size_t i = lean_usize_of_nat(i_nat);\
     ctyp value;\
     memcpy(&value, lean_pod_BytesView_unwrap(bv)->ptr + i, sizeof(ctyp));\
     return value;\
 }\
-LEAN_EXPORT ctyp lean_pod_readBytesViewOffElUnal_##ltyp(size_t sz, b_lean_obj_arg a, b_lean_obj_arg bv, size_t i) {\
+LEAN_EXPORT ctyp lean_pod_readBytesViewOffElUnal_##ltyp(b_lean_obj_arg sz, b_lean_obj_arg a, b_lean_obj_arg bv, b_lean_obj_arg i_nat) {\
+    size_t i = lean_usize_of_nat(i_nat);\
     ctyp value;\
     memcpy(&value, lean_pod_BytesView_unwrap(bv)->ptr + i * sizeof(ctyp), sizeof(ctyp));\
     return value;\
@@ -70,13 +76,15 @@ LEAN_EXPORT ctyp lean_pod_readBytesView_##ltyp(b_lean_obj_arg bv) {\
     memcpy(&value, LEAN_POD_ASSUME_ALIGNED(p, ctyp), sizeof(ctyp));\
     return value;\
 }\
-LEAN_EXPORT ctyp lean_pod_readBytesViewOff_##ltyp(size_t sz, b_lean_obj_arg a, b_lean_obj_arg bv, size_t i) {\
+LEAN_EXPORT ctyp lean_pod_readBytesViewOff_##ltyp(b_lean_obj_arg sz, b_lean_obj_arg a, b_lean_obj_arg bv, b_lean_obj_arg i_nat) {\
+    size_t i = lean_usize_of_nat(i_nat);\
     ctyp value;\
     unsigned char* p = lean_pod_BytesView_unwrap(bv)->ptr + i;\
     memcpy(&value, LEAN_POD_ASSUME_ALIGNED(p, ctyp), sizeof(ctyp));\
     return value;\
 }\
-LEAN_EXPORT ctyp lean_pod_readBytesViewOffEl_##ltyp(size_t sz, b_lean_obj_arg bv, size_t i) {\
+LEAN_EXPORT ctyp lean_pod_readBytesViewOffEl_##ltyp(b_lean_obj_arg sz, b_lean_obj_arg bv, b_lean_obj_arg i_nat) {\
+    size_t i = lean_usize_of_nat(i_nat);\
     ctyp value;\
     unsigned char* p = lean_pod_BytesView_unwrap(bv)->ptr + i * sizeof(ctyp);\
     memcpy(&value, LEAN_POD_ASSUME_ALIGNED(p, ctyp), sizeof(ctyp));\
@@ -87,11 +95,13 @@ LEAN_EXPORT lean_obj_res lean_pod_writeBytesRefUnal_##ltyp(b_lean_obj_arg a, b_l
     memcpy(lean_pod_BytesRef_unwrap(br), &value, sizeof(ctyp));\
     return lean_io_result_mk_ok(lean_box(0));\
 }\
-LEAN_EXPORT lean_obj_res lean_pod_writeBytesRefOffUnal_##ltyp(size_t sz, b_lean_obj_arg a, b_lean_obj_arg br, size_t i, ctyp value, lean_obj_arg st) {\
+LEAN_EXPORT lean_obj_res lean_pod_writeBytesRefOffUnal_##ltyp(b_lean_obj_arg sz, b_lean_obj_arg a, b_lean_obj_arg br, b_lean_obj_arg i_nat, ctyp value, lean_obj_arg st) {\
+    size_t i = lean_usize_of_nat(i_nat);\
     memcpy(lean_pod_BytesRef_unwrap(br) + i, &value, sizeof(ctyp));\
     return lean_io_result_mk_ok(lean_box(0));\
 }\
-LEAN_EXPORT lean_obj_res lean_pod_writeBytesRefOffElUnal_##ltyp(size_t sz, b_lean_obj_arg a, b_lean_obj_arg br, size_t i, ctyp value, lean_obj_arg st) {\
+LEAN_EXPORT lean_obj_res lean_pod_writeBytesRefOffElUnal_##ltyp(b_lean_obj_arg sz, b_lean_obj_arg a, b_lean_obj_arg br, b_lean_obj_arg i_nat, ctyp value, lean_obj_arg st) {\
+    size_t i = lean_usize_of_nat(i_nat);\
     memcpy(lean_pod_BytesRef_unwrap(br) + i * sizeof(ctyp), &value, sizeof(ctyp));\
     return lean_io_result_mk_ok(lean_box(0));\
 }\
@@ -99,12 +109,14 @@ LEAN_EXPORT lean_obj_res lean_pod_writeBytesRef_##ltyp(b_lean_obj_arg br, ctyp v
     memcpy(LEAN_POD_ASSUME_ALIGNED(lean_pod_BytesRef_unwrap(br), ctyp), &value, sizeof(ctyp));\
     return lean_io_result_mk_ok(lean_box(0));\
 }\
-LEAN_EXPORT lean_obj_res lean_pod_writeBytesRefOff_##ltyp(size_t sz, b_lean_obj_arg a, b_lean_obj_arg br, size_t i, ctyp value, lean_obj_arg st) {\
+LEAN_EXPORT lean_obj_res lean_pod_writeBytesRefOff_##ltyp(b_lean_obj_arg sz, b_lean_obj_arg a, b_lean_obj_arg br, b_lean_obj_arg i_nat, ctyp value, lean_obj_arg st) {\
+    size_t i = lean_usize_of_nat(i_nat);\
     unsigned char* p = lean_pod_BytesRef_unwrap(br) + i;\
     memcpy(LEAN_POD_ASSUME_ALIGNED(p, ctyp), &value, sizeof(ctyp));\
     return lean_io_result_mk_ok(lean_box(0));\
 }\
-LEAN_EXPORT lean_obj_res lean_pod_writeBytesRefOffEl_##ltyp(size_t sz, b_lean_obj_arg br, size_t i, ctyp value, lean_obj_arg st) {\
+LEAN_EXPORT lean_obj_res lean_pod_writeBytesRefOffEl_##ltyp(b_lean_obj_arg sz, b_lean_obj_arg br, b_lean_obj_arg i_nat, ctyp value, lean_obj_arg st) {\
+    size_t i = lean_usize_of_nat(i_nat);\
     unsigned char* p = lean_pod_BytesRef_unwrap(br) + i * sizeof(ctyp);\
     memcpy(LEAN_POD_ASSUME_ALIGNED(p, ctyp), &value, sizeof(ctyp));\
     return lean_io_result_mk_ok(lean_box(0));\
