src/lean/Pod/Storable.lean
@@ -3,15 +3,15 @@ import Pod.Lemmas
 namespace Pod
 
 class Storable (α : Type _) where
-  byteSize : USize
+  byteSize : Nat
   alignment : Nat
-  byteSize_gt_zero : byteSize.toNat > 0
-  alignment_dvd_byteSize : ∃ k, byteSize.toNat = alignment * k
+  byteSize_gt_zero : byteSize > 0 := by decide
+  alignment_dvd_byteSize : ∃ k, byteSize = alignment * k := by exists 1
 
 export Storable (byteSize byteSize_gt_zero alignment alignment_dvd_byteSize)
 
 @[reducible]
-def byteSizeArray (α : Type) [Storable α] (n : Nat) : USize := n.toUSize * byteSize α
+def byteSizeArray (α : Type) [Storable α] (n : Nat) : Nat := n * byteSize α
 
 theorem not_alignment_eq_zero {α} [Storable α] : ¬ alignment α = 0 := by
     intro h
@@ -21,25 +21,19 @@ theorem not_alignment_eq_zero {α} [Storable α] : ¬ alignment α = 0 := by
     rw [b, h]
     exact Nat.zero_mul k
 
-def bitWidth {α} [Storable α] : USize := byteSize α * 8
+def bitWidth {α} [Storable α] : Nat := byteSize α * 8
 
 instance : Storable UInt8 where
   byteSize := 1
-  byteSize_gt_zero := Nat.lt_of_lt_of_eq (by constructor) (mod_usize_size_eq 1 $ by decide).symm
   alignment := 1
-  alignment_dvd_byteSize := Exists.intro 1 (mod_usize_size_eq 1 $ by decide)
 
 instance : Storable UInt16 where
   byteSize := 2
-  byteSize_gt_zero := Nat.lt_of_lt_of_eq (by decide) (mod_usize_size_eq 2 $ by decide).symm
   alignment := 2
-  alignment_dvd_byteSize := Exists.intro 1 (mod_usize_size_eq 2 $ by decide)
 
 instance : Storable UInt32 where
   byteSize := 4
-  byteSize_gt_zero := Nat.lt_of_lt_of_eq (by decide) (mod_usize_size_eq 4 $ by decide).symm
   alignment := 4
-  alignment_dvd_byteSize := Exists.intro 1 (mod_usize_size_eq 4 $ by decide)
 
 @[extern "lean_pod_UInt64_getAlignment"]
 private
@@ -47,11 +41,10 @@ opaque UInt64.getAlignment : @& Unit → { n : Nat // n = 4 ∨ n = 8 } := λ _ 
 
 instance : Storable UInt64 where
   byteSize := 8
-  byteSize_gt_zero := Nat.lt_of_lt_of_eq (by decide) (mod_usize_size_eq 8 $ by decide).symm
   alignment := (UInt64.getAlignment ()).val
   alignment_dvd_byteSize := match (UInt64.getAlignment ()).property with
-    | Or.inl h => Exists.intro 2 $ by show 8 % USize.size = _; rw [h, mod_usize_size_eq 8 $ by decide]
-    | Or.inr h => Exists.intro 1 $ by show 8 % USize.size = _; rw [h, mod_usize_size_eq 8 $ by decide]
+    | Or.inl h => Exists.intro 2 $ by rw [h]
+    | Or.inr h => Exists.intro 1 $ by rw [h]
 
 theorem alignment_UInt64_eq : alignment UInt64 = 4 ∨ alignment UInt64 = 8 :=
   (UInt64.getAlignment ()).property
@@ -72,48 +65,20 @@ opaque Float.getAlignment : @& Unit → { n : Nat // n = 4 ∨ n = 8 } := λ _ �
 
 instance : Storable Float where
   byteSize := 8
-  byteSize_gt_zero := Nat.lt_of_lt_of_eq (by decide) (mod_usize_size_eq 8 $ by decide).symm
   alignment := (Float.getAlignment ()).val
   alignment_dvd_byteSize := match (Float.getAlignment ()).property with
-    | Or.inl h => Exists.intro 2 $ by show 8 % USize.size = _; rw [h, mod_usize_size_eq 8 $ by decide]
-    | Or.inr h => Exists.intro 1 $ by show 8 % USize.size = _; rw [h, mod_usize_size_eq 8 $ by decide]
+    | Or.inl h => Exists.intro 2 $ by rw [h]
+    | Or.inr h => Exists.intro 1 $ by rw [h]
 
 theorem alignment_Float_eq : alignment Float = 4 ∨ alignment Float = 8 :=
   (Float.getAlignment ()).property
 
-theorem offEl_no_overflow {α size} [Storable α] (i : USize)
-  (h : i.toNat * (byteSize α).toNat + (byteSize α).toNat ≤ USize.toNat size) :
-    (i * byteSize α).toNat = i.toNat * (byteSize α).toNat := by
-      apply Nat.mod_eq_of_lt
-      apply Nat.lt_of_le_of_lt
-      · show i.toNat * (byteSize α).toNat + 0 ≤ i.toNat * (byteSize α).toNat + (byteSize α).toNat
-        apply Nat.add_le_add_left
-        exact Nat.zero_le _
-      · exact Nat.lt_of_le_of_lt h size.val.isLt
-
-theorem offEl_aligned {α size} [Storable α] (i : USize)
-  (h : i.toNat * (byteSize α).toNat + (byteSize α).toNat ≤ USize.toNat size) :
-  ∀ m, ∃ n, alignment α * m + (i * byteSize α).toNat = (alignment α) * n := λ m ↦
+theorem offEl_aligned {α} [Storable α] (i : Nat) :
+  ∀ m, ∃ n, alignment α * m + i * byteSize α = (alignment α) * n := λ m ↦
     (alignment_dvd_byteSize (α := α)).elim λ aib h₁ ↦
-      Exists.intro (m + i.toNat * aib) $ by
+      Exists.intro (m + i * aib) $ by
         rewrite [Nat.left_distrib]
         apply congrArg (alignment α * m + ·)
-        rewrite [Nat.mul_comm _ aib, ← Nat.mul_assoc, ← h₁, Nat.mul_comm]
-        rw [offEl_no_overflow i h]
-
-theorem off_lt_usize_size {α size} [Storable α] (i : Nat) (h : i + (byteSize α).toNat ≤ USize.toNat size) :
-  i < USize.size := calc
-    i ≤ i + (byteSize α).toNat := Nat.add_le_add_left (Nat.zero_le _) i
-    _ ≤ size.toNat             := h
-    _ < USize.size             := size.val.isLt
-
-theorem offEl_lt_usize_size {α size} [Storable α] (i : Nat)
-  (h : i * (byteSize α).toNat + (byteSize α).toNat ≤ USize.toNat size) :
-    i < USize.size := calc
-      i = i * 1                                       := Eq.symm (Nat.mul_one i)
-      _ ≤ i * (byteSize α).toNat + 0                  := Nat.mul_le_mul_left i byteSize_gt_zero
-      _ ≤ i * (byteSize α).toNat + (byteSize α).toNat := Nat.add_le_add_left (Nat.zero_le _) _
-      _ ≤ size.toNat                                  := h
-      _ < USize.size                                  := size.val.isLt
+        rw [Nat.mul_comm _ aib, ← Nat.mul_assoc, ← h₁, Nat.mul_comm]
 
 end Pod
