src/lean/Pod/Buffer.lean
@@ -3,20 +3,20 @@ import Pod.BytesRef
 
 namespace Pod
 
-opaque BufferPointed (size : USize) (align : Nat) : NonemptyType
-def Buffer (size : USize) (align : Nat) : Type := (BufferPointed size align).type
+opaque BufferPointed (size align : Nat) : NonemptyType
+def Buffer (size align : Nat) : Type := (BufferPointed size align).type
 instance : Nonempty (Buffer size align) := (BufferPointed size align).property
 
 namespace Buffer 
 
 @[extern "lean_pod_Buffer_allocate"]
-opaque allocate (size : USize) : Buffer size 8
+opaque allocate (size : @& Nat) : Buffer size 8
 
 @[extern "lean_pod_Buffer_allocateClear"]
-opaque allocateClear (size : USize) : Buffer size 8
+opaque allocateClear (size : @& Nat) : Buffer size 8
 
 @[extern "lean_pod_Buffer_view"]
-opaque view {size} {align : @& Nat} (buf : Buffer size align) : BytesView size align
+opaque view {size align : @& Nat} (buf : Buffer size align) : BytesView size align
 
 @[extern "lean_pod_Buffer_withRef"]
-opaque withRef {size} {align : @& Nat} (buf : Buffer size align) (f : ∀{σ}, BytesRefMut σ size align → ST σ Unit) : Buffer size align
+opaque withRef {size align : @& Nat} (buf : Buffer size align) (f : ∀{σ}, BytesRefMut σ size align → ST σ Unit) : Buffer size align
