src/lean/Pod/BytesRef.lean
@@ -11,8 +11,8 @@ inductive Mutability where
 
 variable {σ : Type}
 
-opaque BytesRefPointed (σ : Type) (mutab : Mutability) (size : USize) (align : Nat) : NonemptyType
-def BytesRef (σ : Type) (mutab : Mutability) (size : USize) (align : Nat) : Type := (BytesRefPointed σ mutab size align).type
+opaque BytesRefPointed (σ : Type) (mutab : Mutability) (size align : Nat) : NonemptyType
+def BytesRef (σ : Type) (mutab : Mutability) (size align : Nat) : Type := (BytesRefPointed σ mutab size align).type
 instance {σ mutab size align} : Nonempty (BytesRef σ mutab size align) := (BytesRefPointed σ mutab size align).property
 
 abbrev BytesRefMut (σ : Type) := BytesRef σ .Mutable
@@ -20,49 +20,46 @@ abbrev BytesRefImm (σ : Type) := BytesRef σ .Immutable
 
 /-- Clones array if it is shared. -/
 @[extern "lean_pod_ByteArray_withRef"]
-opaque _root_.ByteArray.withRef (ba : ByteArray) (f : ∀{σ}, BytesRefMut σ ba.size.toUSize 1 → ST σ Unit) : ByteArray
+opaque _root_.ByteArray.withRef (ba : ByteArray) (f : ∀{σ}, BytesRefMut σ ba.size 1 → ST σ Unit) : ByteArray
 
 /-- Clones array if it is shared. -/
 @[extern "lean_pod_ByteArray_withRefEx"]
-opaque _root_.ByteArray.withRefEx (ba : ByteArray) (f : ∀{σ}, BytesRefMut σ ba.size.toUSize 1 → EST ε σ Unit) : Except ε ByteArray
+opaque _root_.ByteArray.withRefEx (ba : ByteArray) (f : ∀{σ}, BytesRefMut σ ba.size 1 → EST ε σ Unit) : Except ε ByteArray
 
 namespace BytesRef
 
 @[extern "lean_pod_BytesRef_weaken"]
-opaque weaken {mutab size} {align0 align1 : @& Nat} (h : ∃ k, align1 * k = align0) :
+opaque weaken {mutab} {size align0 align1 : @& Nat} (h : ∃ k, align1 * k = align0) :
   BytesRef σ mutab size align0 → BytesRef σ mutab size align1
 
 @[extern "lean_pod_BytesRef_imm"]
-opaque imm {mutab size} {align : @& Nat} : BytesRef σ mutab size align → BytesRefImm σ size align
+opaque imm {mutab} {size align : @& Nat} : BytesRef σ mutab size align → BytesRefImm σ size align
 
 @[extern "lean_pod_BytesRef_take"]
-opaque take {mutab size} {align : @& Nat} (bv : BytesRef σ mutab size align)
-  (count : USize) (h : count ≤ size) : BytesRef σ mutab count align
+opaque take {mutab} {size align : @& Nat} (bv : BytesRef σ mutab size align)
+  (count : @& Nat) (h : count ≤ size) : BytesRef σ mutab count align
 
 @[extern "lean_pod_BytesRef_drop"]
 opaque drop {mutab size} {align : @& Nat} (bv : BytesRef σ mutab size align)
-  (count : USize) (h : count ≤ size) : BytesRef σ mutab (size - count) (align.gcd count.toNat)
+  (count : @& Nat) (h : count ≤ size) : BytesRef σ mutab (size - count) (align.gcd count)
 
 @[extern "lean_pod_BytesRef_slice"]
-opaque slice {mutab size} {align : @& Nat} (bv : BytesRef σ mutab size align) (start length : USize)
-  (bounded : start.toNat + length.toNat ≤ size.toNat) : BytesRef σ mutab length (align.gcd start.toNat) :=
-  let «start≤size» : start ≤ size := by
-    apply Nat.le_trans $ Nat.le_sub_of_add_le bounded
-    exact Nat.sub_le size.toNat length.toNat
-  (bv.drop start «start≤size»).take length $ by
-    show length.val ≤ (size.val - start.val).val
-    rw [Fin.toNat_sub_distrib size.val start.val «start≤size»]
-    apply Nat.le_sub_of_add_le
-    rw [Nat.add_comm]
-    exact bounded
+opaque slice {mutab} {size align : @& Nat} (bv : BytesRef σ mutab size align) (start length : @& Nat)
+  (bounded : start + length ≤ size) : BytesRef σ mutab length (align.gcd start) := by
+    apply (bv.drop start _).take length 
+    · apply Nat.le_sub_of_add_le
+      rw [Nat.add_comm]
+      exact bounded
+    · apply Nat.le_trans $ Nat.le_sub_of_add_le bounded
+      exact Nat.sub_le size length
 
 /--
 Read all bytes into a `ByteArray`.
 -/
 @[extern "lean_pod_BytesRef_toByteArray"]
-opaque toByteArray {mutab size} {align : @& Nat} (bv : @& BytesRef σ mutab size align) : ST σ ByteArray
+opaque toByteArray {mutab} {size align : @& Nat} (bv : @& BytesRef σ mutab size align) : ST σ ByteArray
 
 @[extern "lean_pod_BytesRef_copyView"]
-opaque copyView {size} {a1 a2 : @& Nat} (dst : @& BytesRefMut σ size a1) (src : @& BytesView size a2) : ST σ Unit
+opaque copyView {size a1 a2 : @& Nat} (dst : @& BytesRefMut σ size a1) (src : @& BytesView size a2) : ST σ Unit
 
 end Pod.BytesRef
