src/lean/Pod/ReadBytes.lean
@@ -5,128 +5,93 @@ import Pod.BytesView
 namespace Pod
 
 class ReadBytes (α : Type) extends Storable α where
-  readBytesRefOffUnal {σ size align} : BytesRefImm σ size align → (i : USize) →
-    i.toNat + byteSize.toNat ≤ size.toNat → ST σ α
+  readBytesRefOffUnal {σ size align} : BytesRefImm σ size align → (i : Nat) →
+    i + byteSize ≤ size → ST σ α
 
   readBytesRefUnal {σ align} (br : BytesRefImm σ byteSize align) : ST σ α :=
     readBytesRefOffUnal br 0 (Nat.le_of_eq $ Nat.zero_add _)
 
-  readBytesRefOffElUnal {σ size align} (br : BytesRefImm σ size align) (i : USize)
-    (h : i.toNat * byteSize.toNat + byteSize.toNat ≤ size.toNat) : ST σ α :=
-      readBytesRefOffUnal br (i * byteSize) (by rw [offEl_no_overflow i h]; exact h)
+  readBytesRefOffElUnal {σ size align} (br : BytesRefImm σ size align) (i : Nat)
+    (h : i * byteSize + byteSize ≤ size) : ST σ α :=
+      readBytesRefOffUnal br (i * byteSize) h
 
-  readBytesRefOff {σ size align} (br : BytesRefImm σ size align) (i : USize)
-    (h₁ : i.toNat + byteSize.toNat ≤ size.toNat)
-    (h₂ : (∀ m, ∃ n, align * m + i.toNat = alignment * n)) : ST σ α :=
+  readBytesRefOff {σ size align} (br : BytesRefImm σ size align) (i : Nat)
+    (h₁ : i + byteSize ≤ size)
+    (h₂ : (∀ m, ∃ n, align * m + i = alignment * n)) : ST σ α :=
       readBytesRefOffUnal br i h₁
 
   readBytesRef {σ} (br : BytesRefImm σ byteSize alignment) : ST σ α :=
     readBytesRefOff br 0 (Nat.le_of_eq $ Nat.zero_add _) λ m ↦
       Exists.intro m (by rw [Nat.add_comm]; exact Nat.zero_add _)
 
-  readBytesRefOffEl {σ size} (br : BytesRefImm σ size alignment) (i : USize)
-    (h : i.toNat * byteSize.toNat + byteSize.toNat ≤ size.toNat) : ST σ α :=
-      readBytesRefOff br (i * byteSize) (by rw [offEl_no_overflow i h]; exact h) (offEl_aligned i h)
+  readBytesRefOffEl {σ size} (br : BytesRefImm σ size alignment) (i : Nat)
+    (h : i * byteSize + byteSize ≤ size) : ST σ α :=
+      readBytesRefOff br (i * byteSize) h (offEl_aligned i)
 
-  readBytesViewOffUnal {size align} : BytesView size align → (i : USize) →
-    i.toNat + byteSize.toNat ≤ size.toNat → α
+  readBytesViewOffUnal {size align} : BytesView size align → (i : Nat) →
+    i + byteSize ≤ size → α
 
   readBytesViewUnal {align} (bv : BytesView byteSize align) : α :=
     readBytesViewOffUnal bv 0 (Nat.le_of_eq $ Nat.zero_add _)
 
   readBytesViewOffElUnal {size align} (bv : BytesView size align)
-    (i : USize) (h : i.toNat * byteSize.toNat + byteSize.toNat ≤ size.toNat) : α :=
-      readBytesViewOffUnal bv (i * byteSize) (by rw [offEl_no_overflow i h]; exact h)
+    (i : Nat) (h : i * byteSize + byteSize ≤ size) : α :=
+      readBytesViewOffUnal bv (i * byteSize) h
 
-  readBytesViewOff {size align} : BytesView size align → (i : USize) →
-    i.toNat + byteSize.toNat ≤ size.toNat →
-    (∀ m, ∃ n, align * m + i.toNat = alignment * n) → α
+  readBytesViewOff {size align} : BytesView size align → (i : Nat) →
+    i + byteSize ≤ size →
+    (∀ m, ∃ n, align * m + i = alignment * n) → α
 
   readBytesView (bv : BytesView byteSize alignment) : α :=
     readBytesViewOff bv 0 (Nat.le_of_eq $ Nat.zero_add _) λ m ↦
       Exists.intro m (by rw [Nat.add_comm]; exact Nat.zero_add _)
 
   readBytesViewOffEl {size} (bv : BytesView size alignment)
-    (i : USize) (h : i.toNat * byteSize.toNat + byteSize.toNat ≤ size.toNat) : α :=
-      readBytesViewOff bv (i * byteSize) (by rw [offEl_no_overflow i h]; exact h) (offEl_aligned i h)
-
+    (i : Nat) (h : i * byteSize + byteSize ≤ size) : α :=
+      readBytesViewOff bv (i * byteSize) h (offEl_aligned i)
 
 def BytesRef.getUnal {α σ align} [ReadBytes α] (br : BytesRefImm σ (byteSize α) align) : ST σ α :=
   ReadBytes.readBytesRefUnal br
 
-def BytesRef.ugetOffUnal {α σ size align} [ReadBytes α] (br : BytesRefImm σ size align) (i : USize)
-  (h₁ : i.toNat + (byteSize α).toNat ≤ size.toNat) : ST σ α :=
+def BytesRef.getOffUnal {α σ size align} [ReadBytes α] (br : BytesRefImm σ size align) (i : Nat)
+  (h₁ : i + (byteSize α) ≤ size) : ST σ α :=
     ReadBytes.readBytesRefOffUnal br i h₁
 
-def BytesRef.getOffUnal {α σ size align} [ReadBytes α] (br : BytesRefImm σ size align) (i : Nat)
-  (h₁ : i + (byteSize α).toNat ≤ size.toNat) : ST σ α :=
-    ReadBytes.readBytesRefOffUnal br ⟨i, off_lt_usize_size i h₁⟩ h₁
-
-def BytesRef.ugetOffElUnal {α σ size align} [ReadBytes α] (br : BytesRefImm σ size align)
-  (i : USize) (h : i.toNat * (byteSize α).toNat + (byteSize α).toNat ≤ size.toNat) : ST σ α :=
-    ReadBytes.readBytesRefOffElUnal br i h
-
 def BytesRef.getOffElUnal {α σ size align} [ReadBytes α] (br : BytesRefImm σ size align)
-  (i : Nat) (h : i * (byteSize α).toNat + (byteSize α).toNat ≤ size.toNat) : ST σ α :=
-    ReadBytes.readBytesRefOffElUnal br ⟨i, offEl_lt_usize_size i h⟩ h
+  (i : Nat) (h : i * (byteSize α) + (byteSize α) ≤ size) : ST σ α :=
+    ReadBytes.readBytesRefOffElUnal br i h
 
 def BytesRef.get {α σ} [ReadBytes α] (br : BytesRefImm σ (byteSize α) (alignment α)) : ST σ α :=
   ReadBytes.readBytesRef br
 
-def BytesRef.ugetOff {α σ size align} [ReadBytes α] (br : BytesRefImm σ size align) (i : USize)
-  (h₁ : i.toNat + (byteSize α).toNat ≤ size.toNat)
-  (h₂ : ∀ m, ∃ n, align * m + i.toNat = alignment α * n) : ST σ α :=
+def BytesRef.getOff {α σ size align} [ReadBytes α] (br : BytesRefImm σ size align) (i : Nat)
+  (h₁ : i + (byteSize α) ≤ size)
+  (h₂ : ∀ m, ∃ n, align * m + i = alignment α * n) : ST σ α :=
     ReadBytes.readBytesRefOff br i h₁ h₂
 
-def BytesRef.getOff {α σ size align} [ReadBytes α] (br : BytesRefImm σ size align) (i : Nat)
-  (h₁ : i + (byteSize α).toNat ≤ size.toNat)
-  (h₂ : ∀ m, ∃ n, align * m + i = alignment α * n) : ST σ α :=
-    ReadBytes.readBytesRefOff br ⟨i, off_lt_usize_size i h₁⟩ h₁ h₂
-
-def BytesRef.ugetOffEl {α σ size} [ReadBytes α] (br : BytesRefImm σ size (alignment α))
-  (i : USize) (h : i.toNat * (byteSize α).toNat + (byteSize α).toNat ≤ size.toNat) : ST σ α :=
-    ReadBytes.readBytesRefOffEl br i h
-
 def BytesRef.getOffEl {α σ size} [ReadBytes α] (br : BytesRefImm σ size (alignment α))
-  (i : Nat) (h : i * (byteSize α).toNat + (byteSize α).toNat ≤ size.toNat) : ST σ α :=
-    ReadBytes.readBytesRefOffEl br ⟨i, offEl_lt_usize_size i h⟩ h
+  (i : Nat) (h : i * (byteSize α) + (byteSize α) ≤ size) : ST σ α :=
+    ReadBytes.readBytesRefOffEl br i h
 
 def BytesView.getUnal {α align} [ReadBytes α] (bv : BytesView (byteSize α) align) : α :=
   ReadBytes.readBytesViewUnal bv
 
-def BytesView.ugetOffUnal {α size align} [ReadBytes α] (bv : BytesView size align) (i : USize)
-  (h₁ : i.toNat + (byteSize α).toNat ≤ size.toNat) : α :=
+def BytesView.getOffUnal {α size align} [ReadBytes α] (bv : BytesView size align) (i : Nat)
+  (h₁ : i + (byteSize α) ≤ size) : α :=
     ReadBytes.readBytesViewOffUnal bv i h₁
 
-def BytesView.getOffUnal {α size align} [ReadBytes α] (bv : BytesView size align) (i : Nat)
-  (h₁ : i + (byteSize α).toNat ≤ size.toNat) : α :=
-    ReadBytes.readBytesViewOffUnal bv ⟨i, off_lt_usize_size i h₁⟩ h₁
-
-def BytesView.ugetOffElUnal {α size align} [ReadBytes α] (bv : BytesView size align)
-  (i : USize) (h : i.toNat * (byteSize α).toNat + (byteSize α).toNat ≤ size.toNat) : α :=
-    ReadBytes.readBytesViewOffElUnal bv i h
-
 def BytesView.getOffElUnal {α size align} [ReadBytes α] (bv : BytesView size align)
-  (i : Nat) (h : i * (byteSize α).toNat + (byteSize α).toNat ≤ size.toNat) : α :=
-    ReadBytes.readBytesViewOffElUnal bv ⟨i, offEl_lt_usize_size i h⟩ h
+  (i : Nat) (h : i * (byteSize α) + (byteSize α) ≤ size) : α :=
+    ReadBytes.readBytesViewOffElUnal bv i h
 
 def BytesView.get {α} [ReadBytes α] (bv : BytesView (byteSize α) (alignment α)) : α :=
   ReadBytes.readBytesView bv
 
-def BytesView.ugetOff {α size align} [ReadBytes α] (bv : BytesView size align) (i : USize)
-  (h₁ : i.toNat + (byteSize α).toNat ≤ size.toNat)
-  (h₂ : ∀ m, ∃ n, align * m + i.toNat = alignment α * n) : α :=
+def BytesView.getOff {α size align} [ReadBytes α] (bv : BytesView size align) (i : Nat)
+  (h₁ : i + (byteSize α) ≤ size)
+  (h₂ : ∀ m, ∃ n, align * m + i = alignment α * n) : α :=
     ReadBytes.readBytesViewOff bv i h₁ h₂
 
-def BytesView.getOff {α size align} [ReadBytes α] (bv : BytesView size align) (i : Nat)
-  (h₁ : i + (byteSize α).toNat ≤ size.toNat)
-  (h₂ : ∀ m, ∃ n, align * m + i = alignment α * n) : α :=
-    ReadBytes.readBytesViewOff bv ⟨i, off_lt_usize_size i h₁⟩ h₁ h₂
-
-def BytesView.ugetOffEl {α size} [ReadBytes α] (bv : BytesView size (alignment α))
-  (i : USize) (h : i.toNat * (byteSize α).toNat + (byteSize α).toNat ≤ size.toNat) : α :=
-    ReadBytes.readBytesViewOffEl bv i h
-
 def BytesView.getOffEl {α size} [ReadBytes α] (bv : BytesView size (alignment α))
-  (i : Nat) (h : i * (byteSize α).toNat + (byteSize α).toNat ≤ size.toNat) : α :=
-    ReadBytes.readBytesViewOffEl bv ⟨i, offEl_lt_usize_size i h⟩ h
+  (i : Nat) (h : i * (byteSize α) + (byteSize α) ≤ size) : α :=
+    ReadBytes.readBytesViewOffEl bv i h
