src/lean/Pod/WriteBytes.lean
@@ -4,72 +4,51 @@ import Pod.BytesRef
 namespace Pod
 
 class WriteBytes (α : Type) extends Storable α where
-  writeBytesRefOffUnal {σ size align} : BytesRefMut σ size align → (i : USize) → α →
-    i.toNat + byteSize.toNat ≤ size.toNat → ST σ Unit
+  writeBytesRefOffUnal {σ size align} : BytesRefMut σ size align → (i : Nat) → α →
+    i + byteSize ≤ size → ST σ Unit
 
   writeBytesRefUnal {σ align} (br : BytesRefMut σ byteSize align) (value : α) : ST σ Unit :=
     writeBytesRefOffUnal br 0 value (Nat.le_of_eq $ Nat.zero_add _)
 
-  writeBytesRefOffElUnal {σ size align} (br : BytesRefMut σ size align) (i : USize) (value : α)
-    (h : i.toNat * byteSize.toNat + byteSize.toNat ≤ size.toNat) : ST σ Unit :=
-      writeBytesRefOffUnal br (i * byteSize) value (by rw [offEl_no_overflow i h]; exact h)
+  writeBytesRefOffElUnal {σ size align} (br : BytesRefMut σ size align) (i : Nat) (value : α)
+    (h : i * byteSize + byteSize ≤ size) : ST σ Unit :=
+      writeBytesRefOffUnal br (i * byteSize) value h
 
-  writeBytesRefOff {σ size align} : BytesRefMut σ size align → (i : USize) → α →
-    i.toNat + byteSize.toNat ≤ size.toNat →
-    (∀ m, ∃ n, align * m + i.toNat = alignment * n) → ST σ Unit
+  writeBytesRefOff {σ size align} : BytesRefMut σ size align → (i : Nat) → α →
+    i + byteSize ≤ size →
+    (∀ m, ∃ n, align * m + i = alignment * n) → ST σ Unit
 
   writeBytesRef {σ} (br : BytesRefMut σ byteSize alignment) (value : α) : ST σ Unit :=
     writeBytesRefOff br 0 value (Nat.le_of_eq $ Nat.zero_add _) λ m ↦
       Exists.intro m (by rw [Nat.add_comm]; exact Nat.zero_add _)
 
-  writeBytesRefOffEl {σ size} (br : BytesRefMut σ size alignment) (i : USize) (value : α)
-    (h : i.toNat * byteSize.toNat + byteSize.toNat ≤ size.toNat) : ST σ Unit :=
-      writeBytesRefOff br (i * byteSize) value (by rw [offEl_no_overflow i h]; exact h) (offEl_aligned i h)
+  writeBytesRefOffEl {σ size} (br : BytesRefMut σ size alignment) (i : Nat) (value : α)
+    (h : i * byteSize + byteSize ≤ size) : ST σ Unit :=
+      writeBytesRefOff br (i * byteSize) value h (offEl_aligned i)
 
 def BytesRef.setUnal {α σ align} [WriteBytes α] (br : BytesRefMut σ (byteSize α) align) (value : α) : ST σ Unit :=
   WriteBytes.writeBytesRefUnal br value
 
-def BytesRef.usetOffUnal {α σ size align} [WriteBytes α]
-  (br : BytesRefMut σ size align) (i : USize) (value : α)
-  (h₁ : i.toNat + (byteSize α).toNat ≤ size.toNat) : ST σ Unit :=
-    WriteBytes.writeBytesRefOffUnal br i value h₁
-
 def BytesRef.setOffUnal {α σ size align} [WriteBytes α]
   (br : BytesRefMut σ size align) (i : Nat) (value : α)
-  (h₁ : i + (byteSize α).toNat ≤ size.toNat) : ST σ Unit :=
-    WriteBytes.writeBytesRefOffUnal br ⟨i, off_lt_usize_size i h₁⟩ value h₁
-
-def BytesRef.usetOffElUnal {α σ size align} [WriteBytes α]
-  (br : BytesRefMut σ size align) (i : USize) (value : α)
-  (h : i.toNat * (byteSize α).toNat + (byteSize α).toNat ≤ size.toNat) : ST σ Unit :=
-    WriteBytes.writeBytesRefOffElUnal br i value h
+  (h₁ : i + (byteSize α) ≤ size) : ST σ Unit :=
+    WriteBytes.writeBytesRefOffUnal br i value h₁
 
 def BytesRef.setOffElUnal {α σ size align} [WriteBytes α]
   (br : BytesRefMut σ size align) (i : Nat) (value : α)
-  (h : i * (byteSize α).toNat + (byteSize α).toNat ≤ size.toNat) : ST σ Unit :=
-    WriteBytes.writeBytesRefOffElUnal br ⟨i, offEl_lt_usize_size i h⟩ value h
+  (h : i * (byteSize α) + (byteSize α) ≤ size) : ST σ Unit :=
+    WriteBytes.writeBytesRefOffElUnal br i value h
 
 def BytesRef.set {α σ} [WriteBytes α] (br : BytesRefMut σ (byteSize α) (alignment α)) (value : α) : ST σ Unit :=
   WriteBytes.writeBytesRef br value
 
-def BytesRef.usetOff {α σ size align} [WriteBytes α]
-  (br : BytesRefMut σ size align) (i : USize) (value : α)
-  (h₁ : i.toNat + (byteSize α).toNat ≤ size.toNat)
-  (h₂ : ∀ m, ∃ n, align * m + i.toNat = alignment α * n) : ST σ Unit :=
-    WriteBytes.writeBytesRefOff br i value h₁ h₂
-
 def BytesRef.setOff {α σ size align} [WriteBytes α]
   (br : BytesRefMut σ size align) (i : Nat) (value : α)
-  (h₁ : i + (byteSize α).toNat ≤ size.toNat)
+  (h₁ : i + (byteSize α) ≤ size)
   (h₂ : ∀ m, ∃ n, align * m + i = alignment α * n) : ST σ Unit :=
-    WriteBytes.writeBytesRefOff br ⟨i, off_lt_usize_size i h₁⟩ value h₁ h₂
-
-def BytesRef.usetOffEl {α σ size} [WriteBytes α]
-  (br : BytesRefMut σ size (alignment α)) (i : USize) (value : α)
-  (h : i.toNat * (byteSize α).toNat + (byteSize α).toNat ≤ size.toNat) : ST σ Unit :=
-    WriteBytes.writeBytesRefOffEl br i value h
+    WriteBytes.writeBytesRefOff br i value h₁ h₂
 
 def BytesRef.setOffEl {α σ size} [WriteBytes α]
   (br : BytesRefMut σ size (alignment α)) (i : Nat) (value : α)
-  (h : i * (byteSize α).toNat + (byteSize α).toNat ≤ size.toNat) : ST σ Unit :=
-    WriteBytes.writeBytesRefOffEl br ⟨i, offEl_lt_usize_size i h⟩ value h
+  (h : i * (byteSize α) + (byteSize α) ≤ size) : ST σ Unit :=
+    WriteBytes.writeBytesRefOffEl br i value h
